EvmCompiler/Assembly.lean
@@ -1,5 +1,5 @@
 import EvmCompiler.Assembly.Syntax
 import EvmCompiler.Assembly.Assembler
+import EvmCompiler.Assembly.Accepted
 import EvmCompiler.Assembly.Semantics
 import EvmCompiler.Assembly.Preservation
-
